src/ProbabilisticProgramming/Quantifier.dfy
@@ -13,12 +13,12 @@ module Quantifier {
   ghost predicate AlmostSurely(p: Random.Bitstream -> bool) {
     var e := iset s | p(s);
     && e in Random.eventSpace
-    && Random.Prob(e) == 1.0
+    && Random.prob(e) == 1.0
   }
 
   ghost predicate WithPosProb(p: Random.Bitstream -> bool) {
     var e := iset s | p(s);
     && e in Random.eventSpace
-    && Random.Prob(e) != 0.0
+    && Random.prob(e) != 0.0
   }
 }
